More attempst

code/hash/Hacl.SHA2.fst
@@ -13,6 +13,9 @@ open Spec.Hash.Helpers
 
 friend Spec.SHA2
 
+(** Top-level constant arrays for the various SHA2 algorithms. *)
+
+(* NOTE: we don't have monotonicity yet so there will be various assumes. *)
 let h224 = B.gcmalloc_of_list HS.root C.h224_l
 let h256 = B.gcmalloc_of_list HS.root C.h256_l
 let h384 = B.gcmalloc_of_list HS.root C.h384_l
@@ -21,25 +24,51 @@ let h512 = B.gcmalloc_of_list HS.root C.h512_l
 let k224_256 = B.gcmalloc_of_list HS.root C.k224_256_l
 let k384_512 = B.gcmalloc_of_list HS.root C.k384_512_l
 
+(* We believe it'll be hard to get, "for free", within this module:
+     readonly h224 /\ writable client_state ==> disjoint h224 client_state
+   so, instead, we require the client to do a little bit of reasoning to show
+   that their buffers are disjoint from our top-level readonly state. *)
+
+(* The total footprint of our morally readonly data. *)
 let static_fp =
   M.loc_union
-    (M.loc_union (M.loc_buffer k224_256) (M.loc_buffer k384_512))
+    (M.loc_union (M.loc_addr_of_buffer k224_256) (M.loc_addr_of_buffer k384_512))
     (M.loc_union
-      (M.loc_union (M.loc_buffer h224) (M.loc_buffer h256))
-      (M.loc_union (M.loc_buffer h384) (M.loc_buffer h512)))
+      (M.loc_union (M.loc_addr_of_buffer h224) (M.loc_addr_of_buffer h256))
+      (M.loc_union (M.loc_addr_of_buffer h384) (M.loc_addr_of_buffer h512)))
 
-let recall_static_fp (): ST.Stack unit
+let loc_in (l: M.loc) (h: HS.mem) =
+  M.(loc_not_unused_in h `loc_includes` l)
+
+(* A useful lemma for clients, to be called at any time before performing an
+   allocation, hence giving them "for free" that their allocation is disjoint from
+   our top-level arrays. *)
+val recall_static_fp: unit -> ST.Stack unit
   (requires (fun _ -> True))
   (ensures (fun h0 _ h1 ->
     M.(modifies loc_none h0 h1) /\
-    M.live h1 static_fp))
-=
+    static_fp `loc_in` h1))
+
+let recall_static_fp () =
   B.recall h224;
   B.recall h256;
   B.recall h384;
   B.recall h512;
   B.recall k224_256;
-  B.recall k384_512
+  B.recall k384_512;
+  let h = ST.get () in
+  assert (M.loc_union
+    (M.loc_union (M.loc_addr_of_buffer k224_256) (M.loc_addr_of_buffer k384_512))
+    (M.loc_union
+      (M.loc_union (M.loc_addr_of_buffer h224) (M.loc_addr_of_buffer h256))
+      (M.loc_union (M.loc_addr_of_buffer h384) (M.loc_addr_of_buffer h512))) `loc_in` h);
+  admit ()
+
+(* This succeeds: *)
+(* let test (): ST.St unit =
+  recall_static_fp ();
+  let b = B.malloc HS.root 0ul 1ul in
+  assert M.(loc_disjoint (loc_addr_of_buffer b) static_fp) *)
 
 let alloca a () =
   [@ inline_let ]
@@ -60,12 +89,11 @@ let alloca_512: alloca_t SHA2_512 =
   T.(synth_by_tactic (specialize (alloca SHA2_512) [`%alloca]))
 
 let init a s =
-  let open Spec in
   match a with
-  | SHA2_224 -> assign_224 s
-  | SHA2_256 -> assign_256 s
-  | SHA2_384 -> assign_384 s
-  | SHA2_512 -> assign_512 s
+  | SHA2_224 -> B.recall h224; B.blit h224 0ul s 0ul 8ul
+  | SHA2_256 -> B.recall h256; B.blit h256 0ul s 0ul 8ul
+  | SHA2_384 -> B.recall h384; B.blit h384 0ul s 0ul 8ul
+  | SHA2_512 -> B.recall h512; B.blit h512 0ul s 0ul 8ul
 
 let init_224: init_t Spec.SHA2_224 =
   T.(synth_by_tactic (specialize (init Spec.SHA2_224) [`%init]))
